Makefile
@@ -1,0 +1,68 @@
+ROOTS := $(wildcard *.fst)
+
+FSTAR = fstar.exe $(SIL) $(FSTAR_FLAGS)
+FSTAR_FLAGS += --cache_dir obj
+FSTAR_FLAGS += --odir obj
+FSTAR_FLAGS += --warn_error -274
+
+KRML = krml -skip-compilation -skip-makefiles $(KSIL)
+
+all: verify
+
+obj/%.fst.checked: %.fst
+	$(call msg,"CHECK",$<)
+	$(FSTAR) -c $< -o $@
+
+obj/%.krml: obj/%.fst.checked
+	$(call msg,"EXTRACT",$<)
+	$(FSTAR) --codegen krml --extract '*,-FStar.Reflection,-FStar.Tactics,-FStar.List' $< -o $@
+
+%.c %.h &: MOD=$(subst _,.,$(basename $(notdir $<)))
+%.c %.h &: obj/%.krml
+	$(call msg,"KRML",$<)
+	$(KRML) $< -bundle '$(MOD)=*'
+
+.PHONY: clean
+clean:
+	rm -rf obj/
+	rm -f .dep .dep.touch
+
+.PHONY: .force
+.dep.touch: .force
+	mkdir -p $(dir $@)
+	[ -e $@ ] || touch $@
+	find . \( -name '*.fst' -o -name '*.fsti' \) -newer $@ -exec touch $@ \; -quit
+
+.dep: .dep.touch
+	$(call msg, "DEPEND", $(SRC))
+	$(Q)$(FSTAR) --dep full $(ROOTS) --already_cached Prims,FStar,Pulse,PulseCore -o $@
+
+ifneq ($(MAKECMDGOALS),clean)
+ifneq ($(MAKECMDGOALS),echo-fstar)
+include .dep
+endif
+endif
+
+verify: $(ALL_CHECKED_FILES)
+
+.PHONY: echo-fstar
+echo-fstar:
+	@echo $(FSTAR)
+
+.DELETE_ON_ERROR:
+.SECONDARY:
+MAKEFLAGS += --no-builtin-rules
+Q?=@
+SIL?=--silent
+KSIL?=-silent
+RAMON=
+ifneq ($(V),)
+	Q=
+	SIL=
+	KSIL=
+else
+	MAKEFLAGS += -s
+endif
+define msg =
+@printf "   %-14s  %s\n" $(1) $(2)
+endef
